theories/L/Datatypes/LFinType.v
@@ -1,6 +1,5 @@
 From Undecidability.L.Tactics Require Import LTactics GenEncode.
 From Undecidability.L Require Import Datatypes.LNat Functions.EqBool.
-From Undecidability.L Require Import UpToC.
 
 Import Nat.
 Require Export Undecidability.Shared.Libs.PSL.FiniteTypes.FinTypes.
@@ -66,17 +65,4 @@ Lemma size_finType_le (X:finType) (x:X):
 Proof.
   rewrite enc_finType_eq,size_nat_enc. specialize (index_le x). 
   unfold c__natsizeS, c__natsizeO. lia.
-Qed.
-
-
-Lemma size_finType_any_le (X:finType) `{encodable X} (x:X):
-  L_facts.size (enc x) <= maxl (map (fun x => L_facts.size (enc x)) (elem X)).
-Proof.
-  apply maxl_leq. eapply in_map_iff. eauto.
-Qed.
-
-Lemma size_finType_any_le_c (X:finType) `{encodable X}:
-  (fun (x:X) => L_facts.size (enc x)) <=c (fun _ => 1).
-Proof.
-  setoid_rewrite size_finType_any_le. smpl_upToC_solve.
 Qed.
