theories/L/Prelim/MoreBase.v
@@ -80,10 +80,3 @@ Proof.
   rewrite <- IHl,<- H. all:now eauto.
 Qed.
 
-Lemma sumn_map_le_pointwise X (xs:list X) f1 f2:
-  (forall x, x el xs -> f1 x <= f2 x) -> sumn (map f1 xs) <= sumn (map f2 xs).
-Proof.
-  intros Hle. 
-  induction xs. easy.
-  cbn. rewrite Hle. 2:now trivial with list. rewrite IHxs. easy. intros. eauto with list.
-Qed.
