theories/TM/Lifting/Lifting.v
@@ -1,1 +1,0 @@
-From Undecidability.TM.Lifting Require Export LiftTapes LiftAlphabet.
